txn-data-consistency/Serializable_2PC_2PL.thy
@@ -89,6 +89,8 @@ datatype 'v ev = Prepare key txid0 | RLock key 'v txid0 | WLock key 'v "'v optio
   User_Commit cl_id | Cl_Commit cl_id sqn cl_view "'v fingerpr"| Cl_Abort cl_id | Cl_ReadyC cl_id |
   Cl_ReadyA cl_id | Skip2
 
+text \<open>Auxiliary definitions\<close>
+
 definition svr_t'_unchanged where
   "svr_t'_unchanged t k svrss svrss' \<equiv> (\<forall>t'. t' \<noteq> t \<longrightarrow>
      svr_fp (svrss' k) t' = svr_fp (svrss k) t' \<and>
@@ -129,11 +131,35 @@ abbreviation is_locked :: "state_svr \<Rightarrow> bool" where
 abbreviation not_locked :: "state_svr \<Rightarrow> bool" where
   "not_locked svr_st \<equiv> svr_st \<notin> {write_lock, read_lock}"
 
-definition updated_kvs :: "'v global_conf \<Rightarrow> cl_id \<Rightarrow> 'v kv_store" where
-  "updated_kvs s cl \<equiv> (\<lambda>k. update_kv_all_txn
+(*
+definition updated_kvs' :: "'v global_conf \<Rightarrow> cl_id \<Rightarrow> 'v kv_store" where  (* old def *)
+  "updated_kvs' s cl \<equiv> (\<lambda>k. update_kv_all_txn
     (\<lambda>t. cl_state (cls (s \<lparr> cls := (cls s)
       (cl := cls s cl \<lparr> cl_state := cl_committed \<rparr> ) \<rparr>) (get_cl t)))
     (svr_state (svrs s k)) (svr_fp (svrs s k)) (svr_vl (svrs s k)))"
+
+definition updated_kvs :: "'v global_conf \<Rightarrow> cl_id \<Rightarrow> 'v kv_store" where   (* new def *)
+  "updated_kvs s cl \<equiv> (\<lambda>k. update_kv_all_txn
+    (\<lambda>t. if get_cl t = cl then cl_committed else cl_state (cls s (get_cl t)))
+    (svr_state (svrs s k)) (svr_fp (svrs s k)) (svr_vl (svrs s k)))"
+
+lemma "updated_kvs' s cl k = updated_kvs s cl k" 
+  apply (auto simp add: updated_kvs'_def updated_kvs_def)
+  apply (rule arg_cong[where f="\<lambda>Z. update_kv_all_txn Z (svr_state (svrs s k)) (svr_fp (svrs s k)) (svr_vl (svrs s k))"])
+  apply auto
+  done 
+
+text \<open>Direct definition of the updated client view, equivalent to length of @{term \<open>updated_kvs\<close>}\<close>
+
+definition updated_cl_view :: "'v global_conf \<Rightarrow> cl_id \<Rightarrow> key \<Rightarrow> nat" where
+  "updated_cl_view gs cl = (\<lambda>k. 
+      if (\<exists>t. (get_cl t = cl \<or> cl_state (cls gs (get_cl t)) = cl_committed) \<and> 
+              svr_state (svrs gs k) t = write_lock) 
+      then Suc (length (svr_vl (svrs gs k))) 
+      else length (svr_vl (svrs gs k)))"
+*)
+
+text \<open>Events' transition relations\<close>
 
 definition prepare where
   "prepare k t s s' \<equiv>
@@ -169,8 +195,7 @@ definition acq_wr_lock where \<comment>\<open>Write Lock acquired\<close>
 definition acq_no_lock where \<comment>\<open>No Lock needed\<close>
   "acq_no_lock k t s s' \<equiv>
     cl_state (cls s (get_cl t)) = cl_prepared
-    \<and> svr_fp (svrs s' k) t W = None
-    \<and> svr_fp (svrs s' k) t R = None
+    \<and> svr_fp (svrs s' k) t = Map.empty
     \<and> svr_state_trans s k s' t prepared no_lock"
 
 definition nok where \<comment>\<open>Lock not available\<close>
@@ -207,33 +232,35 @@ definition user_commit where
     \<and> cl_view (cls s' cl) = cl_view (cls s cl)
     \<and> svr_cl_cl'_unchanged cl s s'"
 
-definition cl_commit' where
-  "cl_commit' cl sn u'' F s s' \<equiv>
+definition cl_commit where
+  "cl_commit cl sn u'' F s s' \<equiv>
     sn = cl_sn (cls s cl) \<and>
-    u'' = length o (kvs_of_gs s) \<and>
+    u'' = length o kvs_of_gs s \<and>
     F = (\<lambda>k. svr_fp (svrs s k) (get_txn cl s)) \<and>
     cl_state (cls s cl) = cl_prepared \<and>
     (\<forall>k. is_locked (svr_state (svrs s k) (get_txn cl s))) \<and>
     cl_state (cls s' cl) = cl_committed \<and>
     cl_sn (cls s' cl) = cl_sn (cls s cl) \<and>
-    cl_view (cls s' cl) = length o (updated_kvs s cl) \<and>
+    cl_view (cls s' cl) = length o update_kv (Tn_cl sn cl) F (view_of_cl_view u'') (kvs_of_gs s) \<and>
     svr_cl_cl'_unchanged cl s s'"
 
-definition cl_commit where        (* chsp: new def *)
-  "cl_commit cl sn u'' F s s' \<equiv>
+(*
+definition cl_commit' where        (* chsp: new/old def *)
+  "cl_commit' cl sn u'' F s s' \<equiv>
     sn = cl_sn (cls s cl) \<and>
-    u'' = length o (kvs_of_gs s) \<and>
+    u'' = length o kvs_of_gs s \<and>
     F = (\<lambda>k. svr_fp (svrs s k) (get_txn cl s)) \<and>
     cl_state (cls s cl) = cl_prepared \<and>
     (\<forall>k. is_locked (svr_state (svrs s k) (get_txn cl s))) \<and>
     s' = s\<lparr> cls := (cls s)(cl := (cls s cl)
-              \<lparr> cl_state := cl_committed, cl_view := length o (updated_kvs s cl) \<rparr>) \<rparr>"
+              \<lparr> cl_state := cl_committed, cl_view := updated_cl_view s cl \<rparr>) \<rparr>"
 
-lemma "cl_commit cl sn u'' F s s' \<longleftrightarrow> cl_commit' cl sn u'' F s s'"
+lemma cl_commit_defs_equiv:
+  "cl_commit cl sn u'' F s s' \<longleftrightarrow> cl_commit' cl sn u'' F s s'"
   apply (auto simp add: cl_commit'_def cl_commit_def cl_unchanged_defs)
   apply (induct s, induct s', auto)
   done
-
+*)
 
 definition cl_abort where
   "cl_abort cl s s' \<equiv>
