txn-data-consistency/Serializable_2PC_2PL_Invariant_Proofs.thy
@@ -1,0 +1,670 @@
+section \<open>2PC-2PL: Invariant Proofs\<close>
+
+theory Serializable_2PC_2PL_Invariant_Proofs
+  imports Serializable_2PC_2PL
+begin
+
+subsection \<open>Auxiliary definitions and basic lemmas\<close>
+
+fun not_cl_commit :: "'a ev \<Rightarrow> bool" where
+  "not_cl_commit (Cl_Commit cl sn u'' F) = False" |
+  "not_cl_commit _ = True"
+
+lemma not_not_cl_commit [simp]: "\<not>not_cl_commit e \<longleftrightarrow> (\<exists>cl sn u'' F. e = Cl_Commit cl sn u'' F)" 
+  by (auto elim: not_cl_commit.elims)
+
+
+lemma view_of_cl_view_length [simp]: "view_of_cl_view (length \<circ> K) = full_view o K"
+  by (simp add: view_of_cl_view_def full_view_def o_def)
+
+
+
+subsection \<open>Invariants about future and past transactions\<close>
+
+definition TIDFutureKm where
+  "TIDFutureKm s cl \<longleftrightarrow> (\<forall>n k. n > cl_sn (cls s cl) \<longrightarrow> svr_state (svrs s k) (Tn_cl n cl) = working)"
+
+lemmas TIDFutureKmI = TIDFutureKm_def[THEN iffD2, rule_format]
+lemmas TIDFutureKmE[elim] = TIDFutureKm_def[THEN iffD1, elim_format, rule_format]
+
+lemma reach_tidfuturekm [simp, dest]: "reach tps s \<Longrightarrow> TIDFutureKm s cl"
+proof(induction s arbitrary: cl rule: reach.induct)
+  case (reach_init s)
+  then show ?case
+  by (auto simp add: TIDFutureKm_def tps_defs tid_match_def)
+next
+  case (reach_trans s e s')
+  then show ?case 
+  proof (cases e)
+    case (Prepare x31 x32)
+    then show ?thesis using reach_trans
+      apply (auto simp add: tps_trans_defs svr_unchanged_defs tid_match_def TIDFutureKm_def)
+      subgoal for n k apply (cases "(Tn_cl n x) = x32"; cases "k = x31", auto) done.
+  next
+    case (RLock x41 x42 x43)
+    then show ?thesis using reach_trans
+      apply (auto simp add: tps_trans_defs svr_unchanged_defs TIDFutureKm_def)
+      by (metis state_svr.distinct(1))
+  next
+    case (WLock x51 x52 x53 x54)
+    then show ?thesis using reach_trans
+      apply (auto simp add: tps_trans_defs svr_unchanged_defs TIDFutureKm_def)
+      by (metis state_svr.distinct(1))+
+  next
+    case (NoLock x61 x62)
+    then show ?thesis using reach_trans
+      apply (auto simp add: tps_trans_defs svr_unchanged_defs TIDFutureKm_def)
+      by (metis state_svr.distinct(1))
+  next
+    case (NOK x71 x72)
+    then show ?thesis using reach_trans
+      apply (auto simp add: tps_trans_defs svr_unchanged_defs TIDFutureKm_def)
+      by (metis state_svr.distinct(1))+
+  next
+    case (Commit x81 x82)
+    then show ?thesis using reach_trans
+      apply (auto simp add: tps_trans_defs svr_unchanged_defs TIDFutureKm_def)
+      apply (metis state_svr.distinct(3))
+      apply (metis state_svr.distinct(5))
+      by (metis state_svr.distinct(7))
+  next
+    case (Abort x91 x92)
+    then show ?thesis using reach_trans
+      apply (auto simp add: tps_trans_defs svr_unchanged_defs TIDFutureKm_def)
+      apply (metis state_svr.distinct(3))
+      apply (metis state_svr.distinct(5))
+      apply (metis state_svr.distinct(7))
+      by (metis state_svr.distinct(9))
+  next
+    case (User_Commit x10)
+    then show ?thesis using reach_trans
+      by (auto simp add: tps_trans_defs cl_unchanged_defs TIDFutureKm_def, metis)
+  next
+    case (Cl_Commit x111 x112 x113 x114)
+    then show ?thesis using reach_trans
+      by (auto simp add: tps_trans_defs cl_unchanged_defs TIDFutureKm_def, metis)
+  next
+    case (Cl_Abort x12a)
+    then show ?thesis using reach_trans
+      by (auto simp add: tps_trans_defs cl_unchanged_defs TIDFutureKm_def, metis)
+  next
+    case (Cl_ReadyC x13a)
+    then show ?thesis using reach_trans
+      apply (auto simp add: tps_trans_defs cl_unchanged_defs TIDFutureKm_def)
+      by (metis Suc_lessD)
+  next
+    case (Cl_ReadyA x14)
+    then show ?thesis using reach_trans
+      apply (auto simp add: tps_trans_defs cl_unchanged_defs TIDFutureKm_def)
+      by (metis Suc_lessD)
+  qed simp
+qed
+
+definition TIDPastKm where
+  "TIDPastKm s cl \<longleftrightarrow> (\<forall>n k. n < cl_sn (cls s cl) \<longrightarrow> svr_state (svrs s k) (Tn_cl n cl) \<in> {committed, aborted})"
+
+lemmas TIDPastKmI = TIDPastKm_def[THEN iffD2, rule_format]
+lemmas TIDPastKmE[elim] = TIDPastKm_def[THEN iffD1, elim_format, rule_format]
+
+lemma reach_tidpastkm [simp, dest]: "reach tps s \<Longrightarrow> TIDPastKm s cl"
+proof(induction s arbitrary: cl rule: reach.induct)
+  case (reach_init s)
+  then show ?case
+  by (auto simp add: TIDPastKm_def tps_defs tid_match_def)
+next
+  case (reach_trans s e s')
+  then show ?case 
+  proof (cases e)
+    case (Prepare x31 x32)
+    then show ?thesis using reach_trans
+      apply (auto simp add: tps_trans_defs svr_unchanged_defs TIDPastKm_def)
+      by (metis state_svr.distinct(11) state_svr.distinct(13))
+  next
+    case (RLock x41 x42 x43)
+    then show ?thesis using reach_trans
+      apply (auto simp add: tps_trans_defs svr_unchanged_defs TIDPastKm_def)
+      by (metis state_svr.distinct(23) state_svr.distinct(25))
+  next
+    case (WLock x51 x52 x53 x54)
+    then show ?thesis using reach_trans
+      apply (auto simp add: tps_trans_defs svr_unchanged_defs TIDPastKm_def)
+      by (metis state_svr.distinct(23) state_svr.distinct(25))+
+  next
+    case (NoLock x61 x62)
+    then show ?thesis using reach_trans
+      apply (auto simp add: tps_trans_defs svr_unchanged_defs TIDPastKm_def)
+      by (metis state_svr.distinct(23) state_svr.distinct(25))
+  next
+    case (NOK x71 x72)
+    then show ?thesis using reach_trans
+      apply (auto simp add: tps_trans_defs svr_unchanged_defs TIDPastKm_def)
+      by (metis state_svr.distinct(23) state_svr.distinct(25))+
+  next
+    case (Commit x81 x82)
+    then show ?thesis using reach_trans
+      by (auto simp add: tps_trans_defs svr_unchanged_defs TIDPastKm_def, fastforce+)
+  next
+    case (Abort x91 x92)
+    then show ?thesis using reach_trans
+      by (auto simp add: tps_trans_defs svr_unchanged_defs TIDPastKm_def, fastforce+)
+  next
+    case (User_Commit x10)
+    then show ?thesis using reach_trans
+      by (auto simp add: tps_trans_defs cl_unchanged_defs TIDPastKm_def, metis)
+  next
+    case (Cl_Commit x111 x112 x113 x114)
+    then show ?thesis using reach_trans
+      by (auto simp add: tps_trans_defs cl_unchanged_defs TIDPastKm_def, metis)
+  next
+    case (Cl_Abort x12a)
+    then show ?thesis using reach_trans
+      by (auto simp add: tps_trans_defs cl_unchanged_defs TIDPastKm_def, metis)
+  next
+    case (Cl_ReadyC x13a)
+    then show ?thesis using reach_trans
+      apply (auto simp add: tps_trans_defs cl_unchanged_defs TIDPastKm_def)
+        by (metis less_antisym)
+  next
+    case (Cl_ReadyA x14)
+    then show ?thesis using reach_trans
+      apply (auto simp add: tps_trans_defs cl_unchanged_defs TIDPastKm_def)
+        by (metis less_antisym)
+  qed auto
+qed
+
+
+subsection \<open>Locking Invariants\<close>
+
+subsubsection \<open>Read lock invariant\<close>
+
+definition RLockInv where
+  "RLockInv s k \<longleftrightarrow> (\<forall>t. svr_state (svrs s k) t = read_lock \<longrightarrow> (\<forall>t. svr_state (svrs s k) t \<noteq> write_lock))"
+
+lemmas RLockInvI = RLockInv_def[THEN iffD2, rule_format]
+lemmas RLockInvE[elim] = RLockInv_def[THEN iffD1, elim_format, rule_format]
+
+lemma reach_rlock [simp, dest]: "reach tps s \<Longrightarrow> RLockInv s k"
+proof(induction s arbitrary: k rule: reach.induct)
+  case (reach_init s)
+  then show ?case
+  by (auto simp add: RLockInv_def tps_defs)
+next
+  case (reach_trans s e s')
+  then show ?case
+  proof (induction e)
+    case (Prepare x1 x2)
+    then show ?case using reach_trans
+      apply (auto simp add: tps_trans_defs svr_unchanged_defs RLockInv_def)
+      by (metis state_svr.distinct(15) state_svr.distinct(17))
+  next
+    case (RLock x1 x2 x3)
+    then show ?case using reach_trans
+      apply (auto simp add: tps_trans_defs svr_unchanged_defs RLockInv_def)
+      by (metis state_svr.distinct(27))
+  next
+    case (WLock x1 x2 x3 x4)
+    then show ?case using reach_trans
+      apply (auto simp add: tps_trans_defs svr_unchanged_defs RLockInv_def)
+      by (metis state_svr.distinct(27))+
+  next
+    case (NoLock x1 x2)
+    then show ?case using reach_trans
+      apply (auto simp add: tps_trans_defs svr_unchanged_defs RLockInv_def)
+      by (metis state_svr.distinct(30) state_svr.distinct(38))
+  next
+    case (NOK x1 x2)
+    then show ?case using reach_trans
+      apply (auto simp add: tps_trans_defs svr_unchanged_defs RLockInv_def)
+      by (metis state_svr.distinct(31) state_svr.distinct(39))
+      (*apply (metis state_svr.distinct(31))
+      apply (metis state_svr.distinct(31))
+      by (metis state_svr.distinct(40))*)
+  next
+    case (Commit x1 x2)
+    then show ?case using reach_trans
+      apply (auto simp add: tps_trans_defs svr_unchanged_defs RLockInv_def)
+      apply (metis state_svr.distinct(42))
+      apply (metis state_svr.distinct(34))
+      by (metis state_svr.distinct(34) state_svr.distinct(42))
+  next
+    case (Abort x1 x2)
+    then show ?case using reach_trans
+      apply (auto simp add: tps_trans_defs svr_unchanged_defs RLockInv_def)
+      apply (metis state_svr.distinct(44))
+      apply (metis state_svr.distinct(36))
+      apply (metis state_svr.distinct(36) state_svr.distinct(44))
+      by (metis state_svr.distinct(35) state_svr.distinct(44))
+  qed (auto simp add: tps_trans_defs cl_unchanged_defs RLockInv_def)
+qed
+
+
+subsubsection \<open>Write lock invariant\<close>
+
+definition WLockInv where
+  "WLockInv s k \<longleftrightarrow> (\<forall>t. svr_state (svrs s k) t \<noteq> write_lock) \<or> (\<exists>!t. svr_state (svrs s k) t = write_lock)"
+
+lemmas WLockInvI = WLockInv_def[THEN iffD2, rule_format]
+lemmas WLockInvE[elim] = WLockInv_def[THEN iffD1, elim_format, rule_format]
+
+lemma reach_wlock [simp, dest]: "reach tps s \<Longrightarrow> WLockInv s k"
+proof(induction s arbitrary: k rule: reach.induct)
+  case (reach_init s)
+  then show ?case
+  by (auto simp add: WLockInv_def tps_defs)
+next
+  case (reach_trans s e s')
+  then show ?case
+  proof (cases e)
+    case (Prepare x31 x32)
+    then show ?thesis using reach_trans
+      apply (auto simp add: tps_trans_defs svr_unchanged_defs WLockInv_def)
+      by (metis state_svr.distinct(17))
+  next
+    case (RLock x41 x42 x43)
+    then show ?thesis using reach_trans
+      apply (auto simp add: tps_trans_defs svr_unchanged_defs WLockInv_def)
+      by (metis state_svr.distinct(27))
+  next
+    case (WLock x51 x52 x53 x54)
+    then show ?thesis using reach_trans
+      apply (auto simp add: tps_trans_defs svr_unchanged_defs WLockInv_def)
+      by metis+
+  next
+    case (NoLock x61 x62)
+    then show ?thesis using reach_trans
+      apply (auto simp add: tps_trans_defs svr_unchanged_defs WLockInv_def)
+      by (metis state_svr.distinct(37))
+  next
+    case (NOK x71 x72)
+    then show ?thesis using reach_trans
+      apply (auto simp add: tps_trans_defs svr_unchanged_defs WLockInv_def)
+      by (metis state_svr.distinct(39))+
+  next
+    case (Commit x81 x82)
+    then show ?thesis using reach_trans
+      apply (auto simp add: tps_trans_defs svr_unchanged_defs WLockInv_def)
+      by (metis state_svr.distinct(41))+
+  next
+    case (Abort x91 x92)
+    then show ?thesis using reach_trans
+      apply (auto simp add: tps_trans_defs svr_unchanged_defs WLockInv_def)
+      by (metis state_svr.distinct(43))+
+  qed (auto simp add: tps_trans_defs cl_unchanged_defs WLockInv_def)
+qed
+
+lemma the_wr_tI:
+  assumes "svr_state (svrs s k) t = write_lock"
+      and "WLockInv s k"
+  shows "the_wr_t (svr_state (svrs s k)) = t"
+  using assms
+  by blast
+
+
+subsection \<open>Invariants for fingerprint, knowing the lock (svrs status)\<close>
+
+definition RLockFpInv where
+  "RLockFpInv s k \<longleftrightarrow> (\<forall>t. svr_state (svrs s k) t = read_lock \<longrightarrow>
+    svr_fp (svrs s k) t W = None \<and>
+    svr_fp (svrs s k) t R \<noteq> None)"
+
+lemmas RLockFpInvI = RLockFpInv_def[THEN iffD2, rule_format]
+lemmas RLockFpInvE[elim] = RLockFpInv_def[THEN iffD1, elim_format, rule_format]
+
+lemma reach_rlockfp [simp, dest]: "reach tps s \<Longrightarrow> RLockFpInv s k"
+proof(induction s arbitrary: k rule: reach.induct)
+  case (reach_init s)
+  then show ?case by (auto simp add: RLockFpInv_def tps_defs)
+next
+  case (reach_trans s e s')
+  then show ?case 
+  proof (cases e)
+    case (Prepare x31 x32)
+    then show ?thesis using reach_trans
+      apply (auto simp add: tps_trans_defs svr_unchanged_defs RLockFpInv_def)
+      by (metis state_svr.distinct(15))+
+  next
+    case (RLock x41 x42 x43)
+    then show ?thesis using reach_trans
+      apply (auto simp add: tps_trans_defs svr_unchanged_defs RLockFpInv_def)
+      by metis+
+  next
+    case (WLock x51 x52 x53 x54)
+    then show ?thesis using reach_trans
+      apply (auto simp add: tps_trans_defs svr_unchanged_defs RLockFpInv_def)
+      by (metis state_svr.distinct(27))+
+  next
+    case (NoLock x61 x62)
+    then show ?thesis using reach_trans
+      apply (auto simp add: tps_trans_defs svr_unchanged_defs RLockFpInv_def)
+      by (metis state_svr.distinct(29))+
+  next
+    case (NOK x71 x72)
+    then show ?thesis using reach_trans
+      apply (auto simp add: tps_trans_defs svr_unchanged_defs RLockFpInv_def)
+      by (metis state_svr.distinct(31))+
+  next
+    case (Commit x81 x82)
+    then show ?thesis using reach_trans
+      apply (auto simp add: tps_trans_defs svr_unchanged_defs RLockFpInv_def)
+      by (metis state_svr.distinct(33))+
+  next
+    case (Abort x91 x92)
+    then show ?thesis using reach_trans
+      apply (auto simp add: tps_trans_defs svr_unchanged_defs RLockFpInv_def)
+      by (metis state_svr.distinct(35))+
+  qed (auto simp add: tps_trans_defs cl_unchanged_defs RLockFpInv_def)
+qed
+
+definition WLockFpInv where
+  "WLockFpInv s k \<longleftrightarrow> (\<forall>t. svr_state (svrs s k) t = write_lock \<longrightarrow> svr_fp (svrs s k) t W \<noteq> None)"
+
+lemmas WLockFpInvI = WLockFpInv_def[THEN iffD2, rule_format]
+lemmas WLockFpInvE[elim] = WLockFpInv_def[THEN iffD1, elim_format, rule_format]
+
+lemma reach_wlockfp [simp, dest]: "reach tps s \<Longrightarrow> WLockFpInv s k"
+proof(induction s arbitrary: k rule: reach.induct)
+  case (reach_init s)
+  then show ?case by (auto simp add: WLockFpInv_def tps_defs)
+next
+  case (reach_trans s e s')
+  then show ?case 
+  proof (cases e)
+    case (Prepare x31 x32)
+    then show ?thesis using reach_trans
+      apply (auto simp add: tps_trans_defs svr_unchanged_defs WLockFpInv_def)
+      by (metis state_svr.distinct(17))
+  next
+    case (RLock x41 x42 x43)
+    then show ?thesis using reach_trans
+      apply (auto simp add: tps_trans_defs svr_unchanged_defs WLockFpInv_def)
+      by (metis state_svr.distinct(27))
+  next
+    case (WLock x51 x52 x53 x54)
+    then show ?thesis using reach_trans
+      apply (auto simp add: tps_trans_defs svr_unchanged_defs WLockFpInv_def)
+      by metis+
+  next
+    case (NoLock x61 x62)
+    then show ?thesis using reach_trans
+      apply (auto simp add: tps_trans_defs svr_unchanged_defs WLockFpInv_def)
+      by (metis state_svr.distinct(37))
+  next
+    case (NOK x71 x72)
+    then show ?thesis using reach_trans
+      apply (auto simp add: tps_trans_defs svr_unchanged_defs WLockFpInv_def)
+      by (metis state_svr.distinct(39))
+  next
+    case (Commit x81 x82)
+    then show ?thesis using reach_trans
+      apply (auto simp add: tps_trans_defs svr_unchanged_defs WLockFpInv_def)
+      by (metis state_svr.distinct(41))+
+  next
+    case (Abort x91 x92)
+    then show ?thesis using reach_trans
+      apply (auto simp add: tps_trans_defs svr_unchanged_defs WLockFpInv_def)
+      by (metis state_svr.distinct(43))+
+  qed (auto simp add: tps_trans_defs cl_unchanged_defs WLockFpInv_def)
+qed
+
+
+definition NoLockFpInv where
+  "NoLockFpInv s k \<longleftrightarrow> (\<forall>t. svr_state (svrs s k) t = no_lock \<longrightarrow> svr_fp (svrs s k) t = Map.empty)"
+
+lemmas NoLockFpInvI = NoLockFpInv_def[THEN iffD2, rule_format]
+lemmas NoLockFpInvE[elim] = NoLockFpInv_def[THEN iffD1, elim_format, rule_format]
+lemmas NoLockFpInvD = NoLockFpInv_def[THEN iffD1, rule_format, rotated 1]
+
+lemma reach_nolockfp [simp, dest]: "reach tps s \<Longrightarrow> NoLockFpInv s k"
+proof(induction s arbitrary: k rule: reach.induct)
+  case (reach_init s)
+  then show ?case by (auto simp add: NoLockFpInv_def tps_defs)
+next
+  case (reach_trans s e s')
+  then show ?case 
+  proof (cases e)
+    case (Prepare x31 x32)
+    then show ?thesis using reach_trans
+      by (auto simp add: tps_trans_defs svr_unchanged_defs NoLockFpInv_def)
+         (metis state_svr.distinct(19))+
+  next
+    case (RLock x41 x42 x43)
+    then show ?thesis using reach_trans
+      by (auto simp add: tps_trans_defs svr_unchanged_defs NoLockFpInv_def)
+         (metis state_svr.distinct(29))+
+  next
+    case (WLock x51 x52 x53 x54)
+    then show ?thesis using reach_trans
+      by (auto simp add: tps_trans_defs svr_unchanged_defs NoLockFpInv_def)
+         (metis state_svr.simps(38))+
+  next
+    case (NoLock k t)
+    then show ?thesis using reach_trans
+      by (auto simp add: tps_trans_defs svr_unchanged_defs NoLockFpInv_def) (metis)
+  next
+    case (NOK x71 x72)
+    then show ?thesis using reach_trans
+      by (auto simp add: tps_trans_defs svr_unchanged_defs NoLockFpInv_def)
+         (metis state_svr.distinct(45))+
+  next
+    case (Commit x81 x82)
+    then show ?thesis using reach_trans
+      by (auto simp add: tps_trans_defs svr_unchanged_defs NoLockFpInv_def)
+         (metis state_svr.distinct(47))+
+  next
+    case (Abort x91 x92)
+    then show ?thesis using reach_trans
+      by (auto simp add: tps_trans_defs svr_unchanged_defs NoLockFpInv_def)
+         (metis state_svr.simps(50))+
+  qed (auto simp add: tps_trans_defs cl_unchanged_defs NoLockFpInv_def)
+qed
+
+lemma the_wr_t_fp:
+  assumes "\<And>k. WLockInv s k"
+    and "\<And>k. WLockFpInv s k"
+    and "svr_state (svrs s k) t = write_lock"
+  shows "svr_fp (svrs s k) (the_wr_t (svr_state (svrs s k))) W \<noteq> None"
+  using assms 
+  by (auto simp add: WLockInv_def WLockFpInv_def the_wr_tI)
+
+
+
+subsection \<open>Lemmas for unchanged elements in svrs\<close>
+
+lemma svr_vl_eq_all_k:
+  assumes "svr_vl (svrs s' k) = svr_vl (svrs s k)"
+    and "other_insts_unchanged k (svrs s) (svrs s')"
+  shows "\<forall>k. svr_vl (svrs s' k) = svr_vl (svrs s k)"
+  using assms by (auto simp add: other_insts_unchanged_def)
+
+lemma eq_for_all_k: 
+  assumes "f (svrs s' k) t = f (svrs s k) t"
+    and "\<And>k'. k' \<noteq> k \<Longrightarrow> svrs s' k' = svrs s k'"
+    and "\<And>t'. t' \<noteq> t \<Longrightarrow> f (svrs s' k) t' = f (svrs s k) t'"
+  shows "f (svrs s' k) = f (svrs s k)"
+  using assms
+  apply (auto simp add: fun_eq_iff) 
+  subgoal for t' by (cases "t' = t", simp_all)
+  done
+
+lemma eq_for_all_cl:
+  assumes "f (cls s' cl) = f (cls s cl)"
+    and "\<forall>cl'. cl' \<noteq> cl \<longrightarrow> cls s' cl' = cls s cl'"
+  shows "f (cls s' cl') = f (cls s cl')"
+  using assms 
+  by (cases "cl' = cl"; simp)
+
+lemma other_sn_idle:  
+  assumes "TIDFutureKm s cl" and "TIDPastKm s cl"
+    and "get_cl t = cl" and "get_sn t \<noteq> cl_sn (cls s cl)"
+  shows "\<And>k. svr_state (svrs s k) t \<in> {working, committed, aborted}"
+  using assms
+  apply (auto simp add: TIDFutureKm_def TIDPastKm_def)
+  apply (cases "get_sn t > cl_sn (cls s cl)")
+  apply (metis txid0.collapse)
+  by (metis linorder_neqE_nat txid0.collapse)
+
+
+
+subsubsection \<open>Invariants about KV store\<close>
+
+definition KVSNonEmp where
+  "KVSNonEmp s \<longleftrightarrow> (\<forall>k. svr_vl (svrs s k) \<noteq> [])"
+
+lemmas KVSNonEmpI = KVSNonEmp_def[THEN iffD2, rule_format]
+lemmas KVSNonEmpE[elim] = KVSNonEmp_def[THEN iffD1, elim_format, rule_format]
+
+lemma reach_kvs_non_emp [simp, dest]: "reach tps s \<Longrightarrow> KVSNonEmp s"
+proof(induction s rule: reach.induct)
+  case (reach_init s)
+  then show ?case
+    by (auto simp add: KVSNonEmp_def tps_defs)
+next
+  case (reach_trans s e s')
+  then show ?case
+  proof (induction e)
+    case (Commit x1 x2)
+    then show ?case using reach_trans 
+      by (auto simp add: KVSNonEmp_def tps_trans_defs svr_unchanged_defs)
+         (metis length_greater_0_conv list.size(3) nat.distinct(1) length_update_kv_key)+
+  qed (auto simp add: KVSNonEmp_def tps_trans_defs unchanged_defs dest!: svr_vl_eq_all_k)
+qed
+
+
+subsubsection \<open>Fingerprint content invariants\<close>
+
+lemma svr_vl_read_commit_eq_lv:
+  assumes "RLockFpInv s k"
+    and "svr_state (svrs s k) t = read_lock"
+    and "svr_state (svrs s' k) t = committed"
+    and "svr_vl (svrs s' k) =
+          update_kv_key t (svr_fp (svrs s k) t) (full_view (svr_vl (svrs s k))) (svr_vl (svrs s k))"
+  shows "v_value (last_version (svr_vl (svrs s' k)) (full_view (svr_vl (svrs s' k)))) =
+         v_value (last_version (svr_vl (svrs s k)) (full_view (svr_vl (svrs s k))))"
+  using assms
+  by (metis RLockFpInv_def max_in_full_view full_view_update_kv_key_no_write update_kv_key_v_value_inv)
+
+
+definition RLockFpContentInv where
+  "RLockFpContentInv s k \<longleftrightarrow> (\<forall>t. svr_state (svrs s k) t = read_lock \<longrightarrow>
+    svr_fp (svrs s k) t R =
+      Some (v_value (last_version (svr_vl (svrs s k)) (full_view (svr_vl (svrs s k))))))"
+
+lemmas RLockFpContentInvI = RLockFpContentInv_def[THEN iffD2, rule_format]
+lemmas RLockFpContentInvE[elim] = RLockFpContentInv_def[THEN iffD1, elim_format, rule_format]
+lemmas RLockFpContentInvD = RLockFpContentInv_def[THEN iffD1, rule_format, rotated 1]
+
+lemma reach_rlockfp_content [simp, dest]: "reach tps s \<Longrightarrow> RLockFpContentInv s k"
+proof(induction s arbitrary: k rule: reach.induct)
+  case (reach_init s)
+  then show ?case by (auto simp add: RLockFpContentInv_def tps_defs)
+next
+  case (reach_trans s e s')
+  then show ?case 
+  proof (cases e)
+    case (Prepare x31 x32)
+    then show ?thesis using reach_trans
+      apply (auto simp add: tps_trans_defs svr_unchanged_defs RLockFpContentInv_def)
+      by (metis state_svr.distinct(15))+
+  next
+    case (RLock x41 x42 x43)
+    then show ?thesis using reach_trans
+      apply (auto simp add: tps_trans_defs svr_unchanged_defs RLockFpContentInv_def)
+      by metis+
+  next
+    case (WLock x51 x52 x53 x54)
+    then show ?thesis using reach_trans
+      apply (auto simp add: tps_trans_defs svr_unchanged_defs RLockFpContentInv_def)
+      by (metis state_svr.distinct(27))+
+  next
+    case (NoLock x61 x62)
+    then show ?thesis using reach_trans
+      apply (auto simp add: tps_trans_defs svr_unchanged_defs RLockFpContentInv_def)
+      by (metis state_svr.distinct(29))+
+  next
+    case (NOK x71 x72)
+    then show ?thesis using reach_trans
+      apply (auto simp add: tps_trans_defs svr_unchanged_defs RLockFpContentInv_def)
+      by (metis state_svr.distinct(31))+
+  next
+    case (Commit x81 x82)
+    then show ?thesis using reach_trans svr_vl_read_commit_eq_lv[of s x81 x82 s']
+      apply (auto simp add: tps_trans_defs svr_unchanged_defs RLockFpContentInv_def del: disjE)
+      by (smt (verit, best) NoLockFpInv_def RLockInv_def reach_nolockfp reach_rlock 
+              state_svr.distinct(33) update_kv_key_nop)
+  next
+    case (Abort x91 x92)
+    then show ?thesis using reach_trans
+      apply (auto simp add: tps_trans_defs svr_unchanged_defs RLockFpContentInv_def)
+      by (metis state_svr.distinct(35))+
+  qed (auto simp add: tps_trans_defs cl_unchanged_defs RLockFpContentInv_def)
+qed
+
+
+definition WLockFpContentInv where
+  "WLockFpContentInv s k \<longleftrightarrow> (\<forall>t. svr_state (svrs s k) t = write_lock \<longrightarrow>
+    svr_fp (svrs s k) t R = None \<or>
+    svr_fp (svrs s k) t R =
+      Some (v_value (last_version (svr_vl (svrs s k)) (full_view (svr_vl (svrs s k))))))"
+
+lemmas WLockFpContentInvI = WLockFpContentInv_def[THEN iffD2, rule_format]
+lemmas WLockFpContentInvE[elim] = WLockFpContentInv_def[THEN iffD1, elim_format, rule_format]
+lemmas WLockFpContentInvD = WLockFpContentInv_def[THEN iffD1, rule_format, rotated 1]
+
+lemma reach_wlockfp_content [simp, dest]: "reach tps s \<Longrightarrow> WLockFpContentInv s k"
+proof(induction s arbitrary: k rule: reach.induct)
+  case (reach_init s)
+  then show ?case by (auto simp add: WLockFpContentInv_def tps_defs)
+next
+  case (reach_trans s e s')
+  then show ?case 
+  proof (cases e)
+    case (Prepare x31 x32)
+    then show ?thesis using reach_trans
+      apply (auto simp add: tps_trans_defs svr_unchanged_defs WLockFpContentInv_def)
+      by (metis state_svr.distinct(17))
+  next
+    case (RLock x41 x42 x43)
+    then show ?thesis using reach_trans
+      apply (auto simp add: tps_trans_defs svr_unchanged_defs WLockFpContentInv_def)
+      by (metis state_svr.distinct(27))
+  next
+    case (WLock x51 x52 x53 x54)
+    then show ?thesis using reach_trans
+      apply (auto simp add: tps_trans_defs svr_unchanged_defs WLockFpContentInv_def)
+      by metis+
+  next
+    case (NoLock x61 x62)
+    then show ?thesis using reach_trans
+      apply (auto simp add: tps_trans_defs svr_unchanged_defs WLockFpContentInv_def)
+      by (metis state_svr.distinct(37))
+  next
+    case (NOK x71 x72)
+    then show ?thesis using reach_trans
+      apply (auto simp add: tps_trans_defs svr_unchanged_defs WLockFpContentInv_def)
+      by (metis state_svr.distinct(39))+
+  next
+    case (Commit x81 x82)
+    then show ?thesis using reach_trans
+      apply (auto simp add: tps_trans_defs svr_unchanged_defs WLockFpContentInv_def)
+      apply (metis RLockInv_def reach_rlock state_svr.distinct(41))
+       apply (smt reach_wlock state_svr.distinct(41) the_wr_tI)
+      by (metis NoLockFpInv_def reach_nolockfp update_kv_key_nop)
+  next
+    case (Abort x91 x92)
+    then show ?thesis using reach_trans
+      apply (auto simp add: tps_trans_defs svr_unchanged_defs WLockFpContentInv_def)
+      by (metis state_svr.distinct(43))+
+  qed (auto simp add: tps_trans_defs cl_unchanged_defs WLockFpContentInv_def)
+qed
+
+
+(* TODO: move parameters into invariant definitions *)
+
+abbreviation invariant_list_kvs where
+  "invariant_list_kvs s \<equiv>  KVSNonEmp s \<and> (\<forall>cl. TIDFutureKm s cl) \<and> (\<forall>cl. TIDPastKm s cl) \<and> 
+                           (\<forall>k. RLockInv s k) \<and> (\<forall>k. RLockFpInv s k) \<and> (\<forall>k. RLockFpContentInv s k) \<and>
+                           (\<forall>k. WLockInv s k) \<and> (\<forall>k. WLockFpInv s k) \<and> (\<forall>k. WLockFpContentInv s k) \<and>
+                           (\<forall>k. NoLockFpInv s k)"
+
+
+end
